backends/lean/Aeneas/Std/Scalar/CoreConvertNum.lean
@@ -58,55 +58,55 @@ def FromI64Bool.from (b : Bool) : I64 :=
 def FromI128Bool.from (b : Bool) : I128 :=
   if b then 1#i128 else 0#i128
 
-def FromUsizeU8.from (x : U8) : Usize := ⟨ x.toBitVec.setWidth _ ⟩
-def FromUsizeU16.from (x : U16) : Usize := ⟨ x.toBitVec.setWidth _ ⟩
-def FromUsizeU32.from (x : U32) : Usize := ⟨ x.toBitVec.setWidth _ ⟩
-def FromUsizeUsize.from (x : Usize) : Usize := ⟨ x.toBitVec.setWidth _ ⟩
+def FromUsizeU8.from (x : U8) : Usize := .ofBitVec (x.toBitVec.setWidth _)
+def FromUsizeU16.from (x : U16) : Usize := .ofBitVec (x.toBitVec.setWidth _)
+def FromUsizeU32.from (x : U32) : Usize := .ofBitVec (x.toBitVec.setWidth _)
+def FromUsizeUsize.from (x : Usize) : Usize := .ofBitVec (x.toBitVec.setWidth _)
 
-def FromU8U8.from (x : U8) : U8 := ⟨ x.toBitVec.setWidth _ ⟩
+def FromU8U8.from (x : U8) : U8 := .ofBitVec (x.toBitVec.setWidth _)
 
-def FromU16U8.from (x : U8) : U16 := ⟨ x.toBitVec.setWidth _ ⟩
-def FromU16U16.from (x : U16) : U16 := ⟨ x.toBitVec.setWidth _ ⟩
+def FromU16U8.from (x : U8) : U16 := .ofBitVec (x.toBitVec.setWidth _)
+def FromU16U16.from (x : U16) : U16 := .ofBitVec (x.toBitVec.setWidth _)
 
-def FromU32U8.from (x : U8) : U32 := ⟨ x.toBitVec.setWidth _ ⟩
-def FromU32U16.from (x : U16) : U32 := ⟨ x.toBitVec.setWidth _ ⟩
-def FromU32U32.from (x : U32) : U32 := ⟨ x.toBitVec.setWidth _ ⟩
+def FromU32U8.from (x : U8) : U32 := .ofBitVec (x.toBitVec.setWidth _)
+def FromU32U16.from (x : U16) : U32 := .ofBitVec (x.toBitVec.setWidth _)
+def FromU32U32.from (x : U32) : U32 := .ofBitVec (x.toBitVec.setWidth _)
 
-def FromU64U8.from (x : U8) : U64 := ⟨ x.toBitVec.setWidth _ ⟩
-def FromU64U16.from (x : U16) : U64 := ⟨ x.toBitVec.setWidth _ ⟩
-def FromU64U32.from (x : U32) : U64 := ⟨ x.toBitVec.setWidth _ ⟩
-def FromU64U64.from (x : U64) : U64 := ⟨ x.toBitVec.setWidth _ ⟩
+def FromU64U8.from (x : U8) : U64 := .ofBitVec (x.toBitVec.setWidth _)
+def FromU64U16.from (x : U16) : U64 := .ofBitVec (x.toBitVec.setWidth _)
+def FromU64U32.from (x : U32) : U64 := .ofBitVec (x.toBitVec.setWidth _)
+def FromU64U64.from (x : U64) : U64 := .ofBitVec (x.toBitVec.setWidth _)
 
-def FromU128U8.from (x : U8) : U128 := ⟨ x.toBitVec.setWidth _ ⟩
-def FromU128U16.from (x : U16) : U128 := ⟨ x.toBitVec.setWidth _ ⟩
-def FromU128U32.from (x : U32) : U128 := ⟨ x.toBitVec.setWidth _ ⟩
-def FromU128U64.from (x : U64) : U128 := ⟨ x.toBitVec.setWidth _ ⟩
-def FromU128U128.from (x : U128) : U128 := ⟨ x.toBitVec.setWidth _ ⟩
+def FromU128U8.from (x : U8) : U128 := .ofBitVec (x.toBitVec.setWidth _)
+def FromU128U16.from (x : U16) : U128 := .ofBitVec (x.toBitVec.setWidth _)
+def FromU128U32.from (x : U32) : U128 := .ofBitVec (x.toBitVec.setWidth _)
+def FromU128U64.from (x : U64) : U128 := .ofBitVec (x.toBitVec.setWidth _)
+def FromU128U128.from (x : U128) : U128 := .ofBitVec (x.toBitVec.setWidth _)
 
-def FromIsizeI8.from (x : I8) : Isize := ⟨ x.toBitVec.signExtend _ ⟩
-def FromIsizeI16.from (x : I16) : Isize := ⟨ x.toBitVec.signExtend _ ⟩
-def FromIsizeI32.from (x : I32) : Isize := ⟨ x.toBitVec.signExtend _ ⟩
-def FromIsizeIsize.from (x : Isize) : Isize := ⟨ x.toBitVec.signExtend _ ⟩
+def FromIsizeI8.from (x : I8) : Isize := Isize.ofBitVec (x.toBitVec.signExtend _)
+def FromIsizeI16.from (x : I16) : Isize := Isize.ofBitVec (x.toBitVec.signExtend _)
+def FromIsizeI32.from (x : I32) : Isize := Isize.ofBitVec (x.toBitVec.signExtend _)
+def FromIsizeIsize.from (x : Isize) : Isize := Isize.ofBitVec (x.toBitVec.signExtend _)
 
-def FromI8I8.from (x : I8) : I8 := ⟨ x.toBitVec.signExtend _ ⟩
+def FromI8I8.from (x : I8) : I8 := .ofBitVec (x.toBitVec.signExtend _)
 
-def FromI16I8.from (x : I8) : I16 := ⟨ x.toBitVec.signExtend _ ⟩
-def FromI16I16.from (x : I16) : I16 := ⟨ x.toBitVec.signExtend _ ⟩
+def FromI16I8.from (x : I8) : I16 := .ofBitVec (x.toBitVec.signExtend _)
+def FromI16I16.from (x : I16) : I16 := .ofBitVec (x.toBitVec.signExtend _)
 
-def FromI32I8.from (x : I8) : I32 := ⟨ x.toBitVec.signExtend _ ⟩
-def FromI32I16.from (x : I16) : I32 := ⟨ x.toBitVec.signExtend _ ⟩
-def FromI32I32.from (x : I32) : I32 := ⟨ x.toBitVec.signExtend _ ⟩
+def FromI32I8.from (x : I8) : I32 := .ofBitVec (x.toBitVec.signExtend _)
+def FromI32I16.from (x : I16) : I32 := .ofBitVec (x.toBitVec.signExtend _)
+def FromI32I32.from (x : I32) : I32 := .ofBitVec (x.toBitVec.signExtend _)
 
-def FromI64I8.from (x : I8) : I64 := ⟨ x.toBitVec.signExtend _ ⟩
-def FromI64I16.from (x : I16) : I64 := ⟨ x.toBitVec.signExtend _ ⟩
-def FromI64I32.from (x : I32) : I64 := ⟨ x.toBitVec.signExtend _ ⟩
-def FromI64I64.from (x : I64) : I64 := ⟨ x.toBitVec.signExtend _ ⟩
+def FromI64I8.from (x : I8) : I64 := .ofBitVec (x.toBitVec.signExtend _)
+def FromI64I16.from (x : I16) : I64 := .ofBitVec (x.toBitVec.signExtend _)
+def FromI64I32.from (x : I32) : I64 := .ofBitVec (x.toBitVec.signExtend _)
+def FromI64I64.from (x : I64) : I64 := .ofBitVec (x.toBitVec.signExtend _)
 
-def FromI128I8.from (x : I8) : I128 := ⟨ x.toBitVec.signExtend _ ⟩
-def FromI128I16.from (x : I16) : I128 := ⟨ x.toBitVec.signExtend _ ⟩
-def FromI128I32.from (x : I32) : I128 := ⟨ x.toBitVec.signExtend _ ⟩
-def FromI128I64.from (x : I64) : I128 := ⟨ x.toBitVec.signExtend _ ⟩
-def FromI128I128.from (x : I128) : I128 := ⟨ x.toBitVec.signExtend _ ⟩
+def FromI128I8.from (x : I8) : I128 := .ofBitVec (x.toBitVec.signExtend _)
+def FromI128I16.from (x : I16) : I128 := .ofBitVec (x.toBitVec.signExtend _)
+def FromI128I32.from (x : I32) : I128 := .ofBitVec (x.toBitVec.signExtend _)
+def FromI128I64.from (x : I64) : I128 := .ofBitVec (x.toBitVec.signExtend _)
+def FromI128I128.from (x : I128) : I128 := .ofBitVec (x.toBitVec.signExtend _)
 
 private theorem BitVec.setWidth_toNat_le (m : Nat) (x : BitVec n) (h : n ≤ m) :
   (x.setWidth m).toNat = x.toNat := by
@@ -247,95 +247,95 @@ private theorem bmod_pow2_eq_of_inBounds' (n : ℕ) (x : ℤ) (h : 0 < n ∧ -2 
 @[simp, scalar_tac_simps, simp_scalar_safe, grind =, agrind =]
 theorem FromIsizeI8.from_toInt_eq (x : I8) : (FromIsizeI8.from x).toInt = x.toInt := by
   cases System.Platform.numBits_eq <;>
-  simp only [FromIsizeI8.from, IScalar.toInt, BitVec.signExtend] <;> simp <;>
+  simp only [FromIsizeI8.from, I8.toInt, BitVec.signExtend] <;> simp <;>
   apply bmod_pow2_eq_of_inBounds' _ x.toInt (by scalar_tac)
 
 @[simp, scalar_tac_simps, simp_scalar_safe, grind =, agrind =]
 theorem FromIsizeI16.from_toInt_eq (x : I16) : (FromIsizeI16.from x).toInt = x.toInt := by
   cases System.Platform.numBits_eq <;>
-  simp only [FromIsizeI16.from, IScalar.toInt, BitVec.signExtend] <;> simp <;>
+  simp only [FromIsizeI16.from, I16.toInt, BitVec.signExtend] <;> simp <;>
   apply bmod_pow2_eq_of_inBounds' _ x.toInt (by scalar_tac)
 
 @[simp, scalar_tac_simps, simp_scalar_safe, grind =, agrind =]
 theorem FromIsizeI32.from_toInt_eq (x : I32) : (FromIsizeI32.from x).toInt = x.toInt := by
   cases System.Platform.numBits_eq <;>
-  simp only [FromIsizeI32.from, IScalar.toInt, BitVec.signExtend] <;> simp <;>
+  simp only [FromIsizeI32.from, I32.toInt, BitVec.signExtend] <;> simp <;>
   apply bmod_pow2_eq_of_inBounds' _ x.toInt (by scalar_tac)
 
 @[simp, scalar_tac_simps, simp_scalar_safe, grind =, agrind =]
 theorem FromIsizeIsize.from_toInt_eq (x : Isize) : (FromIsizeIsize.from x).toInt = x.toInt := by
   cases System.Platform.numBits_eq <;>
-  simp only [FromIsizeIsize.from, IScalar.toInt, BitVec.signExtend] <;> simp
+  simp only [FromIsizeIsize.from, Isize.toInt, BitVec.signExtend] <;> simp
 
 @[simp, scalar_tac_simps, simp_scalar_safe, grind =, agrind =]
 theorem FromI8I8.from_toInt_eq (x : I8) : (FromI8I8.from x).toInt = x.toInt := by
-  simp only [FromI8I8.from, IScalar.toInt, BitVec.signExtend]; simp
+  simp only [FromI8I8.from, I8.toInt, BitVec.signExtend]; simp
 
 @[simp, scalar_tac_simps, simp_scalar_safe, grind =, agrind =]
 theorem FromI16I8.from_toInt_eq (x : I8) : (FromI16I8.from x).toInt = x.toInt := by
-  simp only [FromI16I8.from, IScalar.toInt, BitVec.signExtend]; simp
+  simp only [FromI16I8.from, I8.toInt, BitVec.signExtend]; simp
   apply bmod_pow2_eq_of_inBounds' 16 x.toInt (by scalar_tac)
 
 @[simp, scalar_tac_simps, simp_scalar_safe, grind =, agrind =]
 theorem FromI16I16.from_toInt_eq (x : I16) : (FromI16I16.from x).toInt = x.toInt := by
-  simp only [FromI16I16.from, IScalar.toInt, BitVec.signExtend]; simp
+  simp only [FromI16I16.from, I16.toInt, BitVec.signExtend]; simp
 
 @[simp, scalar_tac_simps, simp_scalar_safe, grind =, agrind =]
 theorem FromI32I8.from_toInt_eq (x : I8) : (FromI32I8.from x).toInt = x.toInt := by
-  simp only [FromI32I8.from, IScalar.toInt, BitVec.signExtend]; simp
+  simp only [FromI32I8.from, I8.toInt, BitVec.signExtend]; simp
   apply bmod_pow2_eq_of_inBounds' 32 x.toInt (by scalar_tac)
 
 @[simp, scalar_tac_simps, simp_scalar_safe, grind =, agrind =]
 theorem FromI32I16.from_toInt_eq (x : I16) : (FromI32I16.from x).toInt = x.toInt := by
-  simp only [FromI32I16.from, IScalar.toInt, BitVec.signExtend]; simp
+  simp only [FromI32I16.from, I16.toInt, BitVec.signExtend]; simp
   apply bmod_pow2_eq_of_inBounds' 32 x.toInt (by scalar_tac)
 
 @[simp, scalar_tac_simps, simp_scalar_safe, grind =, agrind =]
 theorem FromI32I32.from_toInt_eq (x : I32) : (FromI32I32.from x).toInt = x.toInt := by
-  simp only [FromI32I32.from, IScalar.toInt, BitVec.signExtend]; simp
+  simp only [FromI32I32.from, I32.toInt, BitVec.signExtend]; simp
 
 @[simp, scalar_tac_simps, simp_scalar_safe, grind =, agrind =]
 theorem FromI64I8.from_toInt_eq (x : I8) : (FromI64I8.from x).toInt = x.toInt := by
-  simp only [FromI64I8.from, IScalar.toInt, BitVec.signExtend]; simp
+  simp only [FromI64I8.from, I8.toInt, BitVec.signExtend]; simp
   apply bmod_pow2_eq_of_inBounds' 64 x.toInt (by scalar_tac)
 
 @[simp, scalar_tac_simps, simp_scalar_safe, grind =, agrind =]
 theorem FromI64I16.from_toInt_eq (x : I16) : (FromI64I16.from x).toInt = x.toInt := by
-  simp only [FromI64I16.from, IScalar.toInt, BitVec.signExtend]; simp
+  simp only [FromI64I16.from, I16.toInt, BitVec.signExtend]; simp
   apply bmod_pow2_eq_of_inBounds' 64 x.toInt (by scalar_tac)
 
 @[simp, scalar_tac_simps, simp_scalar_safe, grind =, agrind =]
 theorem FromI64I32.from_toInt_eq (x : I32) : (FromI64I32.from x).toInt = x.toInt := by
-  simp only [FromI64I32.from, IScalar.toInt, BitVec.signExtend]; simp
+  simp only [FromI64I32.from, I32.toInt, BitVec.signExtend]; simp
   apply bmod_pow2_eq_of_inBounds' 64 x.toInt (by scalar_tac)
 
 @[simp, scalar_tac_simps, simp_scalar_safe, grind =, agrind =]
 theorem FromI64I64.from_toInt_eq (x : I64) : (FromI64I64.from x).toInt = x.toInt := by
-  simp only [FromI64I64.from, IScalar.toInt, BitVec.signExtend]; simp
+  simp only [FromI64I64.from, I64.toInt, BitVec.signExtend]; simp
 
 @[simp, scalar_tac_simps, simp_scalar_safe, grind =, agrind =]
 theorem FromI128I8.from_toInt_eq (x : I8) : (FromI128I8.from x).toInt = x.toInt := by
-  simp only [FromI128I8.from, IScalar.toInt, BitVec.signExtend]; simp
+  simp only [FromI128I8.from, I8.toInt, BitVec.signExtend]; simp
   apply bmod_pow2_eq_of_inBounds' 128 x.toInt (by scalar_tac)
 
 @[simp, scalar_tac_simps, simp_scalar_safe, grind =, agrind =]
 theorem FromI128I16.from_toInt_eq (x : I16) : (FromI128I16.from x).toInt = x.toInt := by
-  simp only [FromI128I16.from, IScalar.toInt, BitVec.signExtend]; simp
+  simp only [FromI128I16.from, I16.toInt, BitVec.signExtend]; simp
   apply bmod_pow2_eq_of_inBounds' 128 x.toInt (by scalar_tac)
 
 @[simp, scalar_tac_simps, simp_scalar_safe, grind =, agrind =]
 theorem FromI128I32.from_toInt_eq (x : I32) : (FromI128I32.from x).toInt = x.toInt := by
-  simp only [FromI128I32.from, IScalar.toInt, BitVec.signExtend]; simp
+  simp only [FromI128I32.from, I32.toInt, BitVec.signExtend]; simp
   apply bmod_pow2_eq_of_inBounds' 128 x.toInt (by scalar_tac)
 
 @[simp, scalar_tac_simps, simp_scalar_safe, grind =, agrind =]
 theorem FromI128I64.from_toInt_eq (x : I64) : (FromI128I64.from x).toInt = x.toInt := by
-  simp only [FromI128I64.from, IScalar.toInt, BitVec.signExtend]; simp
+  simp only [FromI128I64.from, I64.toInt, BitVec.signExtend]; simp
   apply bmod_pow2_eq_of_inBounds' 128 x.toInt (by scalar_tac)
 
 @[simp, scalar_tac_simps, simp_scalar_safe, grind =, agrind =]
 theorem FromI128I128.from_toInt_eq (x : I128) : (FromI128I128.from x).toInt = x.toInt := by
-  simp only [FromI128I128.from, IScalar.toInt, BitVec.signExtend]; simp
+  simp only [FromI128I128.from, I128.toInt, BitVec.signExtend]; simp
 
 @[simp, bvify, grind =, agrind =] theorem FromIsizeI8.from_toBitVec_eq (x : I8) : (FromIsizeI8.from x).toBitVec = x.toBitVec.signExtend _ := by rfl
 
