backends/lean/Aeneas/Std/Scalar/Casts.lean
@@ -26,7 +26,7 @@ run_cmd do
       scalar @[step_pure_def] instance : ScalarCast $(mkIdent ty) «%S» where
         cast x :=
           -- This truncates the integer if the numBits is smaller
-          ⟨ x.toBitVec.zeroExtend %BitWidth ⟩
+          .ofBitVec (x.toBitVec.zeroExtend %BitWidth)
     ))
 
 open Lean in
@@ -37,7 +37,7 @@ run_cmd do
     Lean.Elab.Command.elabCommand (← `(
       scalar @[step_pure_def] instance : ScalarCast $(mkIdent ty) «%S» where
         cast x :=
-          ⟨ x.toBitVec.signExtend %BitWidth ⟩
+          .ofBitVec (x.toBitVec.signExtend %BitWidth)
     ))
 
 section
@@ -74,94 +74,69 @@ section
 end
 
 scalar instance : ScalarCast Bool «%S» where
-  cast x := if x then ⟨ 1#%BitWidth ⟩ else ⟨ 0#%BitWidth ⟩
+  cast x := if x then .ofBitVec (1#%BitWidth) else .ofBitVec (0#%BitWidth)
 
 /-!
 # Casts: Theorems
 -/
 
-/- This theorem allows us not to use bit-vectors when reasoning about casts, if there are no overflows -/
-open Lean in
-set_option hygiene false in
-run_cmd do
-  for ty in [`U8, `U16, `U32, `U64, `U128, `Usize] do
-    Lean.Elab.Command.elabCommand (← `(
-      uscalar theorem $(mkIdent s!"«%S».cast_{ty.toString}_inBounds_spec".toName)
-        (x : $(mkIdent ty)) (h : x.toNat ≤ «%S».max) :
-        lift (ScalarCast.cast «%S» x) ⦃ y => y.toNat = x.toNat ⦄ := by
-        simp only [lift, ScalarCast.cast, BitVec.truncate_eq_setWidth, WP.spec_ok, UScalar.toNat]
-        unfold UScalarTy.numBits
-        simp only [max, BitVec.toNat_setWidth] at *
-        apply Nat.mod_eq_of_lt; scalar_tac
-    ))
+uuscalar
+/-- This theorem allows us not to use bit-vectors when reasoning about casts, if there are no overflows -/
+theorem «%S1».cast_'S2_inBounds_spec
+  (x : «%S2») (h : x.toNat ≤ «%S1».max) :
+  lift (ScalarCast.cast «%S1» x) ⦃ y => y.toNat = x.toNat ⦄ := by
+  simp only [lift, ScalarCast.cast, BitVec.truncate_eq_setWidth, WP.spec_ok, toNat_ofBitVec]
+  simp only [max, BitVec.toNat_setWidth] at *
+  apply Nat.mod_eq_of_lt; scalar_tac
 
-/- This theorem allows us not to use bit-vectors when reasoning about casts, if there are no overflows -/
-open Lean in
-set_option hygiene false in
-run_cmd do
-  for ty in [`U8, `U16, `U32, `U64, `U128, `Usize] do
-    Lean.Elab.Command.elabCommand (← `(
-      iscalar theorem $(mkIdent s!"«%S».cast_{ty.toString}_inBounds_spec".toName)
-        (x : $(mkIdent ty)) (h : x.toNat ≤ «%S».max) :
-        lift (ScalarCast.cast «%S» x) ⦃ y => y.toInt = x.toNat ⦄ := by
-          simp only [lift, ScalarCast.cast, BitVec.truncate_eq_setWidth, WP.spec_ok]
-          simp only [IScalar.toInt, UScalar.toNat]
-          simp only [IScalarTy.numBits]
-          simp only [BitVec.toInt_setWidth, UScalar.toBitVec_toNat] at *
-          have := System.Platform.numBits_eq
-          apply Int.bmod_pow2_eq_of_inBounds' <;> scalar_tac
-    ))
+iuscalar
+/-- This theorem allows us not to use bit-vectors when reasoning about casts, if there are no overflows -/
+theorem «%S1».cast_'S2_inBounds_spec
+  (x : «%S2») (h : x.toNat ≤ «%S1».max) :
+  lift (ScalarCast.cast «%S1» x) ⦃ y => y.toInt = x.toNat ⦄ := by
+    simp only [lift, ScalarCast.cast, BitVec.truncate_eq_setWidth, WP.spec_ok, toInt_ofBitVec]
+    simp only [BitVec.toInt_setWidth, max] at *
+    have := System.Platform.numBits_eq
+    apply Int.bmod_pow2_eq_of_inBounds' <;> scalar_tac
 
-/- This theorem allows us not to use bit-vectors when reasoning about casts, if there are no overflows -/
-open Lean in
-set_option hygiene false in
-run_cmd do
-  for ty in [`I8, `I16, `I32, `I64, `I128, `Isize] do
-    Lean.Elab.Command.elabCommand (← `(
-      iscalar theorem $(mkIdent s!"«%S».cast_{ty.toString}_inBounds_spec".toName)
-      (x : $(mkIdent ty)) (h : «%S».min ≤ x.toInt ∧ x.toInt ≤ «%S».max) :
-        lift (ScalarCast.cast «%S» x) ⦃ y => y.toInt = x.toInt ⦄
-        := by
-        simp only [lift, ScalarCast.cast, BitVec.signExtend, IScalar.toBitVec_toInt_eq, WP.spec_ok]
-        simp only [IScalar.toInt]
-        simp only [IScalarTy.numBits]
-        simp only [min, max, IScalar.toBitVec_toInt_eq, BitVec.toInt_ofInt] at *
-        have := System.Platform.numBits_eq
-        apply Int.bmod_pow2_eq_of_inBounds' <;> scalar_tac
-    ))
+iiscalar
+/-- This theorem allows us not to use bit-vectors when reasoning about casts, if there are no overflows -/
+theorem «%S1».cast_'S2_inBounds_spec
+  (x : «%S2») (h : «%S1».min ≤ x.toInt ∧ x.toInt ≤ «%S1».max) :
+  lift (ScalarCast.cast «%S1» x) ⦃ y => y.toInt = x.toInt ⦄ := by
+  simp only [lift, ScalarCast.cast, BitVec.signExtend, toBitVec_toInt_eq, WP.spec_ok, toInt_ofBitVec]
+  simp only [min, max, BitVec.toInt_ofInt, numBits_eq] at *
+  have := System.Platform.numBits_eq
+  apply Int.bmod_pow2_eq_of_inBounds' <;> scalar_tac
 
-/- This theorem allows us not to use bit-vectors when reasoning about casts, if there are no overflows -/
-open Lean in
-set_option hygiene false in
-run_cmd do
-  for ty in [`I8, `I16, `I32, `I64, `I128, `Isize] do
-    Lean.Elab.Command.elabCommand (← `(
-      uscalar theorem $(mkIdent s!"«%S».cast_{ty.toString}_inBounds_spec".toName)
-        (x : $(mkIdent ty)) (h : 0 ≤ x.toInt ∧ x.toInt ≤ U8.max) :
-        lift (ScalarCast.cast U8 x) ⦃ y => y.toNat = x.toInt ⦄ := by
-        simp only [lift, ScalarCast.cast, BitVec.signExtend, IScalar.toBitVec_toInt_eq, WP.spec_ok]
-        simp only [IScalar.toInt, UScalar.toNat]
-        simp only [UScalarTy.numBits]
-        simp only [Nat.cast_pow, Nat.cast_ofNat,
-          IScalar.toBitVec_toInt_eq, BitVec.toNat_ofInt, Int.ofNat_toNat] at *
-        scalar_tac
-    ))
+uiscalar
+/-- This theorem allows us not to use bit-vectors when reasoning about casts, if there are no overflows -/
+theorem «%S1».cast_'S2_inBounds_spec
+  (x : «%S2») (h : 0 ≤ x.toInt ∧ x.toInt ≤ «%S1».max) :
+  lift (ScalarCast.cast «%S1» x) ⦃ y => y.toNat = x.toInt ⦄ := by
+    simp only [lift, ScalarCast.cast, BitVec.signExtend, IScalar.toBitVec_toInt_eq, WP.spec_ok]
+    simp only [IScalar.toInt, toNat, UScalarTy.numBits]
+    simp only [IScalarTy.I16_numBits_eq, I16.toBitVec_toInt_eq, toBitVec_ofBitVec,
+      BitVec.toNat_ofInt, Nat.reducePow, Nat.cast_ofNat, Int.ofNat_toNat, max] at *
+    rw [numBits_eq] at *
+    rw [max_eq_left (by scalar_tac), Int.emod_eq_of_lt (by scalar_tac) (by scalar_tac)]
+    try scalar_tac
 
 uscalar @[simp, step_pure ScalarCast.cast «%S» b]
 theorem «%S».cast_fromBool_toNat_eq (b : Bool) : (ScalarCast.cast «%S» b).toNat = b.toNat := by
   simp only [ScalarCast.cast]
-  split <;> simp only [UScalar.toNat, *] <;> simp
+  split <;> simp only [*] <;> simp
 
 iscalar @[simp, step_pure ScalarCast.cast «%S» b]
 theorem «%S».cast_fromBool_toInt_eq (b : Bool) : (ScalarCast.cast «%S» b).toInt = b.toInt := by
   simp only [ScalarCast.cast]
   have := System.Platform.numBits_pos
-  split <;> simp only [IScalar.toInt] <;> grind
+  split <;> simp only [toInt] <;> grind
 
 uscalar @[scalar_tac ScalarCast.cast «%S» b]
 theorem «%S».cast_fromBool_bound_eq (b : Bool) : (ScalarCast.cast «%S» b).toNat ≤ 1 := by
   simp only [ScalarCast.cast]
-  split <;> simp only [UScalar.toNat, *] <;> simp
+  split <;> simp only [toNat, *] <;> simp
 
 uscalar @[simp]
 theorem «%S».cast_fromBool_toBitVec_eq (b : Bool) :
@@ -179,24 +154,20 @@ iscalar @[scalar_tac ScalarCast.cast «%S» b]
 theorem «%S».cast_fromBool_bound_eq (b : Bool) :
   0 ≤ (ScalarCast.cast «%S» b).toInt ∧ (ScalarCast.cast «%S» b).toInt ≤ 1 := by
   simp only [ScalarCast.cast]
-  split <;> simp only [IScalar.toInt]
+  split <;> simp only [toInt]
   · have : (1#%BitWidth).toInt = 1 := by
       simp [BitVec.toInt]
       try cases System.Platform.numBits_eq <;> simp [*]
     simp [this]
   · simp
 
-open Lean in
-set_option hygiene false in
-run_cmd do
-  for ty in [`U8, `U16, `U32, `U64, `U128, `Usize] do
-    Lean.Elab.Command.elabCommand (← `(
-      uscalar theorem $(mkIdent s!"{ty.toString}.cast_'S_toNat_eq_mod".toName) (x : $(mkIdent ty)) :
-        (ScalarCast.cast «%S» x).toNat = x.toNat % 2^%BitWidth := by
-        simp only [ScalarCast.cast, UScalar.toNat]
-        simp only [UScalarTy.numBits]
-        simp only [BitVec.truncate_eq_setWidth, BitVec.toNat_setWidth, toBitVec_toNat]
-    ))
+uuscalar theorem «%S1».cast_'S2_toNat_eq_mod (x : «%S1») :
+  (ScalarCast.cast «%S2» x).toNat = x.toNat % 2^%BitWidth2 := by
+  simp only [ScalarCast.cast, toNat]
+  simp only [UScalarTy.numBits]
+  simp only [BitVec.truncate_eq_setWidth,
+    BitVec.toNat_setWidth, toBitVec_toNat, «%S2».toNat_ofBitVec]
+
 
 -- TODO: factor our the casts
 
@@ -285,19 +256,12 @@ run_cmd do
 example (x : U16) : (ScalarCast.cast U32 x).toNat = x.toNat := by simp
 example : (ScalarCast.cast U16 (U32.ofNat 42)).toNat = 42 := by simp
 
-open Lean in
-set_option hygiene false in
-run_cmd do
-  for ty1 in [`I8, `I16, `I32, `I64, `I128, `Isize] do
-    for ty2 in [`I8, `I16, `I32, `I64, `I128, `Isize] do
-      Lean.Elab.Command.elabCommand (← `(
-        theorem $(mkIdent s!"{ty1.toString}.cast_{ty2.toString}_toInt_eq".toName) (x : $(mkIdent ty1)) :
-          (ScalarCast.cast $(mkIdent ty2) x).toInt = Int.bmod x.toInt
-            (2^(Min.min  $(mkIdent (ty2 ++ `numBits)) $(mkIdent (ty1 ++ `numBits)))) := by
-          simp only [ScalarCast.cast, IScalar.toInt, I8.numBits_eq, I16.numBits_eq,
-            I32.numBits_eq, I64.numBits_eq, I128.numBits_eq, Isize.numBits_eq]
-          simp only [IScalarTy.numBits, BitVec.toInt_signExtend]
-      ))
+iiscalar theorem «%S1».cast_'S2_toInt_eq (x : «%S1») :
+  (ScalarCast.cast «%S2» x).toInt = Int.bmod x.toInt
+  (2^(Min.min «%S2».numBits «%S1».numBits)) := by
+    simp only [ScalarCast.cast, toInt, «%S1».numBits_eq, «%S2».numBits_eq]
+    simp only [IScalarTy.numBits, BitVec.toInt_signExtend, «%S2».toInt_ofBitVec,
+      «%S2».toBitVec_ofBitVec]
 
 open Lean in
 set_option hygiene false in
@@ -318,42 +282,27 @@ run_cmd do
           apply Int.bmod_pow2_eq_of_inBounds <;> omega
       ))
 
-open Lean in
-set_option hygiene false in
-run_cmd do
-  for ty1 in [`I8, `I16, `I32, `I64, `I128, `Isize] do
-    for ty2 in [`I8, `I16, `I32, `I64, `I128, `Isize] do
-      Lean.Elab.Command.elabCommand (← `(
-        @[simp]
-        theorem $(mkIdent s!"{ty1.toString}.cast_{ty2.toString}_toInt_mod_pow_inBounds".toName)
-          (x : $(mkIdent ty1))
-          (hMin : -2^($(mkIdent (ty2 ++ `numBits)) - 1) ≤ x.toInt) (hMax : x.toInt < 2^($(mkIdent (ty2 ++ `numBits)) - 1)) :
-          (ScalarCast.cast $(mkIdent ty2) x).toInt = x.toInt := by sorry
-      ))
-
--- theorem I8.ss
---   (x : I8)
---   (hMin : -2^(I16.numBits - 1) ≤ x.toInt) (hMax : x.toInt < 2^(I16.numBits - 1)) :
---   (ScalarCast.cast I16 x).toInt = x.toInt := by
---   simp only [cast_I8_toInt_eq, cast_I16_toInt_eq, cast_I32_toInt_eq,
---     cast_I64_toInt_eq, cast_I128_toInt_eq, cast_Isize_toInt_eq]
---   rw [Int.bmod_eq_of_le_mul_two]
---   by_cases h : I16.numBits ≤ numBits
---   · rw [Nat.min_eq_left h]
---     have : -((2 : Int) ^ (I16.numBits - 1) * 2) ≤ ↑x * 2 := by grind
---     rwa [pow_sub_one_mul I16.numBits_nonzero] at this
---   · rw [Nat.min_eq_right (by grind)]
---     have := (IScalar.hBounds x).1
---     have : -((2 : Int) ^ (numBits - 1) * 2) ≤ ↑x * 2 := by grind [numBits_eq]
---     rwa [pow_sub_one_mul numBits_nonzero] at this
---   by_cases h : I16.numBits ≤ numBits
---   · rw [Nat.min_eq_left h]
---     have : ↑x * 2 < ((2 : Int) ^ (I16.numBits - 1) * 2) := by grind
---     rwa [pow_sub_one_mul I16.numBits_nonzero] at this
---   · rw [Nat.min_eq_right (by grind)]
---     have := (IScalar.hBounds x).1
---     have : ↑x * 2 < ((2 : Int) ^ (numBits - 1) * 2) := by grind [numBits_eq]
---     rwa [pow_sub_one_mul numBits_nonzero] at this
-
+iiscalar @[simp]
+theorem «%S1».cast_'S2_toInt_mod_pow_inBounds (x : «%S1»)
+  (hMin : -2^(«%S2».numBits - 1) ≤ x.toInt) (hMax : x.toInt < 2^(«%S2».numBits - 1)) :
+  (ScalarCast.cast «%S2» x).toInt = x.toInt := by
+  simp only [cast_'S2_toInt_eq]
+  rw [Int.bmod_eq_of_le_mul_two]
+  by_cases h : «%S2».numBits ≤ numBits
+  · rw [Nat.min_eq_left h]
+    have : -((2 : Int) ^ («%S2».numBits - 1) * 2) ≤ ↑x * 2 := by omega
+    rwa [pow_sub_one_mul «%S2».numBits_nonzero] at this
+  · rw [Nat.min_eq_right (by omega)]
+    have := (IScalar.hBounds x).1
+    have : -((2 : Int) ^ (numBits - 1) * 2) ≤ ↑x * 2 := by scalar_tac
+    rwa [pow_sub_one_mul numBits_nonzero] at this
+  by_cases h : «%S2».numBits ≤ numBits
+  · rw [Nat.min_eq_left h]
+    have : ↑x * 2 < ((2 : Int) ^ («%S2».numBits - 1) * 2) := by omega
+    rwa [pow_sub_one_mul «%S2».numBits_nonzero] at this
+  · rw [Nat.min_eq_right (by omega)]
+    have := (IScalar.hBounds x).1
+    have : ↑x * 2 < ((2 : Int) ^ (numBits - 1) * 2) := by scalar_tac
+    rwa [pow_sub_one_mul numBits_nonzero] at this
 
 end Aeneas.Std
